#Optics #PHAS1000 #Y1 
Consider a curved interface between two media of refractive index $n_1$ and $n_2$ such that $n_2 >n_1$ . From Snell’s law we find that an object $P$, at $s$, from the vertex will create an image $P’$, at $s’$ 
![[Screenshot 2025-03-06 092135.png]]
$$\frac{n_{1}}{s}+\frac{n_{2}}{s}=\frac{n_{2}-n_{1}}{s}$$

![[Screenshot 2025-03-06 092254.png]]
$$m=\frac{y'}{y}=\frac{\text{image height}}{\text{object height}}$$
$$\theta_{1}=\frac{y}{s}$$
$$\theta_{2}=\frac{-y'}{s}$$
$$n_{1}\sin \theta_{1}=n_{2}\sin \theta_{2}\Rightarrow n_{1}\theta_{1}=n_{2}\theta_{2}$$
$$n_{1}\frac{y}{s}=n_{2}\left(\frac{-y}{s} \right)$$
$$m=\frac{y'}{y}=-\left( \frac{n_{1}s'}{n_{2}s} \right)$$
A lens has two spherical (or approximately spherical) surfaces with radii of curvature $R_1$ & $R_2$. ($C_1$ and $C_2$ represent the centres of curvature.  

To determine the properties of the lens we need consider refraction at each surface of the lens separately.
![[Screenshot 2025-03-06 093452.png]]
Lenses that are thicker in the middle than towards the edge are known as **convex**
Lenses that are thinner in the middle than towards the edge are known as **concave**


A ray parallel to the principal axis  will be refracted to pass through the focal point.
$$\frac{1}{f}=\left( \frac{n}{n_{air}}-1 \right)\left( \frac{1}{R_{1}}-\frac{1}{R_{2}} \right)$$
![[Screenshot 2025-03-11 091309.png]]

![[Screenshot 2025-03-11 091549.png]]
Principal rays for converging lens:
1. parallel ray: parallel to axis and redirected through F 
2. central ray: passes undeflected through centre of lens  
3. focal ray: passes through F (front focal point) and emerges parallel to axis (since ray paths are reversible). 


![[Screenshot 2025-03-11 091700.png]]

Principal rays for diverging lens
1. parallel ray: parallel to axis and bent as if it came from F  
2. central ray: passes undeflected through centre of lens  
3. focal ray: drawn towards F and emerges parallel to axis  
  
  ![[Screenshot 2025-03-11 092456.png]]
  $$\frac{h}{x}=-\frac{h}{f}\quad\&\quad \frac{h}{f}=\frac{-h'}{x'}$$
$$\Rightarrow \frac{h}{-h'}=\frac{x}{f}\quad\&\quad \frac{h}{-h'}=\frac{f}{x'}\Rightarrow \frac{x}{f}=\frac{f}{x'}$$
Newtons Lens equation
$$xx'=f^2$$
$$s=x+f\quad\&\quad s'=x'+f'$$
$$(s-f)(s'-f)=f^2 \Rightarrow ss'-fs-fs'=0$$
Gauss' Lens equation
$$\frac{1}{s}+\frac{1}{s'}=\frac{1}{f}$$
